# Change of Variable

A core concept in finite elements is that of change of variable.
Immediately, we will use this concept to simplify numerical integration (quadrature), though later this will lead to the idea of parent elements and mapping to/from various configurations utilized within finite element implemntations, for example: *parametric*, *reference*, *current* configurations.

As a simple example of this, let us imagine that we have some function, $f(x)$, that we wish to integrate over the domain $[2, 7]$.
Let us further imagine that we have inherited some code that only supports integration over the domain $[-1, 1]$.
How can we proceed?

Let's imagine that we could define some function, $g(\xi), \xi \in [-1, 1]$, such that $f(x) = g(\xi)$.
That is, when we evaluate $g(\xi)$ at some value in the domain $[-1, 1]$, it evaluates to its "equivalent" value in the function $f(x)$ in the domain $[2, 7]$.
By "equivalent" we mean that if we evaluate $g(\xi)$ at its left boundary, it should be equivalent to evaluating $f(x)$ at its left boundary: $f(2) = g(-1)$.
Similarly evaluating at the right boundaries should be equivalent, $f(7) = g(1)$; evaluating each at their midpoint should be equivalent, $f(4.5) = g(0)$, and so on.

We can do this if we allow for $x$ to be a function (a *mapping*) that allows us to convert some value of $\xi$ into a value for $x$.
We can write this mapping as $x(\xi)$, and the inverse of this mapping as $\xi(x)$.
So how can we write a function that maps between the two domains?  
Let's step through this logically, choosing to modify the domain of $\xi$ so that we determine $x$.

1. Scale $[-1, 1]$ so that it has the same have the same range ("length") as $[2, 7]$.
   - $\left( \frac{7 - 2}{ 1 - ^{-}1} \right) \cdot [-1, 1]$
   - $2.5 \cdot [-1, 1]$
   - $[-1 \cdot 2.5, 1 \cdot 2.5]$
   - $[-2.5, 2.5]$ 
2. Shift the modified domain so that its lower bound equals the other
   - $(2 - ^{-}2.5) + [-2.5, 2.5]$
   - $4.5 + [-2.5, 2.5]$
   - $[-2.5 + 4.5, 2.5 + 4.5]$
   - $[2, 7]$

Ok, so that seems to work! 
But we used words to describe what we wanted to do, and then showed with actual numbers, making it a bit hard to see the algebra that's occurring -- which we want to know so that we can write code to implement the operation.
To help us see the structure, lets replace the numbers with variables:

1. Scale $[\xi_0, \xi_1]$ so that it has the same have the same range ("length") as $[x_0, x_1]$.
   - $\left( \frac{x_1 - x_0}{\xi_1 - \xi_0} \right) \cdot [\xi_0, \xi_1]$
2. Shift the modified domain so that its lower bound equals the other
   - $\left(x_0 - \xi_0\right) + \left( \left( \frac{x_1 - x_0}{\xi_1 - \xi_0} \right) \cdot [\xi_0, \xi_1] \right )$

Now, recognizing that $[\xi_0, \xi_1]$ simply represents two possible values of $\xi$, let's replace the array with $\xi$ and rewrite as a function
$$
x(\xi) = \left(x_0 - \xi_0\right) + \left( \frac{x_1 - x_0}{\xi_1 - \xi_0} \right) \xi
$$

Similarly we can find the inverse function

$$
\xi(x) = \left(\xi_0 - x_0\right) + \left( \frac{\xi_1 - \xi_0}{x_1 - x_0} \right) x
$$

Noting the similar structure of these two mappings, let's now write a function that simply maps from some domain to some other domain using change of variable.

```{python}
#| echo: true
def ChangeOfVariable( from_value, from_domain, to_domain ):
    ## SHIFT TO ZERO
    to_value = from_value - from_domain[0]
    ## SCALE TO EQUAL RANGE
    to_value *= ( to_domain[1] - to_domain[0] ) / ( from_domain[1] - from_domain[0] )
    ## APPLY TO DOMAIN
    to_value += to_domain[0]
    return to_value
```

Let's see this function in action!

```{python}
#| echo: true
from_domain = [-1, 1]
to_domain = [2, 7]
from_values = [-1, -0.5, 0, 0.5, 1]

for from_value in from_values:
    to_value = ChangeOfVariable( from_value, from_domain, to_domain )
    print( f"x({from_value}) = {to_value}" )
```

Now let's see what happens when we use the change of variable in an actual function.  
First let's choose a function defined over $x$ and map it to $\xi$.

```{python}
#| echo: false
from IPython.display import Markdown
import sympy
import spb
sympy.init_printing( use_latex='mathjax', use_unicode=False )
```

```{python}
x_domain = sympy.Array( [2, 7] )
xi_domain = sympy.Array( [-1, 1] )

x = sympy.Symbol( 'x' )
xi = ChangeOfVariable( x, from_domain=xi_domain, to_domain=x_domain )
f = sympy.exp( x ) * sympy.cos( sympy.pi * x )
g = f.subs( x, xi )
```

```{python}
#| echo: false
Markdown( f"$$ f(x) = {sympy.latex( f )}, \\quad x \\in {x_domain}$$\n" + \
          f"$$ \\xi(x) = {sympy.latex( xi )}, \\quad \\xi \\in {xi_domain}$$\n" + \
          f"$$ g(\\xi(x)) = {sympy.latex( g )}$$\n" )
```

```{python}
#| echo: false
p1 = spb.plot( f, ( x, x_domain[0], x_domain[1] ), xlim=[-1, 7], ylabel="$f(x)$", show=False )
p2 = spb.plot( g, ( x, xi_domain[0], xi_domain[1] ), xlim=[-1, 7], ylabel="$g(\\xi(x))$", show=False )
sp1 = spb.plotgrid( p1, p2 )
```

And again on another function, this time using the mapping $x(\xi)$:
```{python}
xi = sympy.Symbol( '\\xi', real = True )
x = ChangeOfVariable( xi, from_domain=x_domain, to_domain=xi_domain )
g = sympy.re( xi**xi ) 
f = g.subs( xi, x )
```

```{python}
#| echo: false
Markdown( f"$$ g(\\xi) = {sympy.latex( g )}, \\quad \\xi \\in {xi_domain}$$\n" + \
          f"$$ x(\\xi) = {sympy.latex( x )}, \\quad x \\in {x_domain}$$\n" + \
          f"$$ f(x(\\xi)) = {sympy.latex( f )}$$\n" )
```

```{python}
#| echo: false
p3 = spb.plot( g, ( xi, xi_domain[0], xi_domain[1] ), xlim=[-1, 7], ylabel="$g(\\xi)$", show=False )
p4 = spb.plot( f, ( xi, x_domain[0], x_domain[1] ), xlim=[-1, 7], ylabel="$f(x(\\xi))$", show=False )
sp2 = spb.plotgrid( p3, p4 )
```